get stateless ml_kernel to build again

hol-light/stateless/ml_kernel/ml_monadScript.sml
@@ -13,6 +13,15 @@ open terminationTheory lcsymtacs;
 
 infix \\ val op \\ = op THEN;
 
+fun auto_prove proof_name (goal,tac) = let
+  val (rest,validation) = tac ([],goal) handle Empty => fail()
+  in if length rest = 0 then validation [] else let
+  in failwith("auto_prove failed for " ^ proof_name) end end
+
+fun D th = let
+  val th = th |> DISCH_ALL |> PURE_REWRITE_RULE [AND_IMP_INTRO]
+  in if is_imp (concl th) then th else DISCH T th end
+
 (* a few basics *)
 
 val _ = (use_full_type_names := false);
@@ -49,7 +58,6 @@ val hol_type_ind = store_thm("hol_type_ind",
   \\ REPEAT STRIP_TAC \\ Q.PAT_ASSUM `!x.bbb` MATCH_MP_TAC
   \\ EVAL_TAC \\ IMP_RES_TAC MEM_hol_type_size \\ DECIDE_TAC);
 
-val LIST_TYPE_def = fetch "-" "LIST_TYPE_def"
 val (*HOL_KERNEL_*)HOL_TYPE_TYPE_def = fetch "-" "HOL_TYPE_TYPE_def"
 
 val LIST_TYPE_NO_CLOSURES = prove(
@@ -298,13 +306,13 @@ val Eval_IMP_PURE = store_thm("Eval_IMP_PURE",
 val HOL_TYPE_TYPE_EXISTS = prove(
   ``?ty v. HOL_TYPE_TYPE ty v``,
   Q.EXISTS_TAC `Tyvar []`
-  \\ fs [fetch "-" "HOL_TYPE_TYPE_def", fetch "-" "LIST_TYPE_def"]);
+  \\ fs [fetch "-" "HOL_TYPE_TYPE_def", LIST_TYPE_def]);
 
 val HOL_TERM_TYPE_EXISTS = prove(
   ``?tm v. HOL_TERM_TYPE tm v``,
   STRIP_ASSUME_TAC HOL_TYPE_TYPE_EXISTS
   \\ Q.EXISTS_TAC `Var [] ty`
-  \\ fs [fetch "-" "HOL_TERM_TYPE_def",fetch "-" "LIST_TYPE_def"]
+  \\ fs [fetch "-" "HOL_TERM_TYPE_def",LIST_TYPE_def]
   \\ Q.EXISTS_TAC `v` \\ FULL_SIMP_TAC std_ss []);
 
 val HOL_STORE_EXISTS = prove(
@@ -320,7 +328,7 @@ val HOL_STORE_EXISTS = prove(
                       the_term_constants := [] ;
                       the_definitions := [] ;
                       the_clash_var := tm |>`
-  \\ FULL_SIMP_TAC (srw_ss()) [fetch "-" "LIST_TYPE_def"]);
+  \\ FULL_SIMP_TAC (srw_ss()) [LIST_TYPE_def]);
 
 val EvalM_ArrowM_IMP = store_thm("EvalM_ArrowM_IMP",
   ``EvalM env (Var x) ((a -M-> b) f) ==>
